added bfr_gen ... generic implementation of BFR based on axiomatic fifos

bfr_gen.v
@@ -12,53 +12,56 @@ Require Import list_utils wf_utils bt bft bft_spec bft_inj fifo_axm bfn_gen.
 
 Set Implicit Arguments.
 
-Section bfr_3q.
+Local Definition fifo_sum { X } (q : fifo (bt X)) := lsum (fifo_list q). 
 
-  Let fifo_3q_sum { X } (q : fifo_3q (bt X)) := lsum (fifo_3q_list q). 
+Section bfr_gen.
 
   Variable (X Y : Type).
 
-  Notation fX := (fifo_3q (bt X)).
-  Notation fY := (fifo_3q (bt Y)).
+  Notation fifo_X := (fifo (bt X)).
+  Notation fifo_Y := (fifo (bt Y)).
 
-  Fixpoint bfr_3q_f (p : fX) (ll : list Y) { struct ll } : 
-            fifo_3q_sum p = length ll
-         -> { q : fY | fifo_3q_list p ~lt rev (fifo_3q_list q) 
-                    /\ bft_f (rev (fifo_3q_list q)) = ll }.
+  Implicit Type (p : fifo_X) (ll : list Y).
+
+  Fixpoint bfr_gen_f p (ll : list Y) { struct ll } : 
+            fifo_sum p = length ll
+         -> { q  | fifo_list p ~lt rev (fifo_list q) 
+                /\ bft_f (rev (fifo_list q)) = ll }.
   Proof.
-    unfold fifo_3q_sum in *.
+    unfold fifo_sum in *.
     refine (match ll with 
-      | nil   => fun Hll => let (q,Hq)   := @fifo_3q_nil_full _ 
+      | nil   => fun Hll => let (q,Hq)   := fifo_nil 
                             in  exist _ q _
-      | y::mm => fun Hll => let (d1,Hd1) := fifo_3q_deq_full p _ 
+      | y::mm => fun Hll => let (d1,Hd1) := fifo_deq p _ 
                             in  _
     end).
     all: cycle 2.
     revert Hd1; refine (match d1 with (t,p1) => _ end); intros Hp1.
     rewrite Hp1 in Hll; simpl in Hll; clear d1.
     revert Hll Hp1; refine (match t with 
-      | leaf x     => fun Hll Hp1 => let (q,Hq)   := bfr_3q_f p1 mm _ in 
-                                     let (q1,Hq1) := fifo_3q_enq_full q (leaf y) 
+      | leaf x     => fun Hll Hp1 => let (q,Hq)   := bfr_gen_f p1 mm _ in 
+                                     let (q1,Hq1) := fifo_enq q (leaf y) 
                                      in  exist _ q1 _
-      | node a x b => fun Hll Hp1 => let (p2,Hp2) := fifo_3q_enq_full p1 a    in
-                                     let (p3,Hp3) := fifo_3q_enq_full p2 b    in
-                                     let (q,Hq)   := bfr_3q_f p3 mm _         in  
-                                     let (d2,Hd2) := fifo_3q_deq_full q _     in _
+      | node a x b => fun Hll Hp1 => let (p2,Hp2) := fifo_enq p1 a     in
+                                     let (p3,Hp3) := fifo_enq p2 b     in
+                                     let (q,Hq)   := bfr_gen_f p3 mm _ in  
+                                     let (d2,Hd2) := fifo_deq q _     
+                                     in  _
     end); auto.
     all: cycle 3.
     revert Hd2; refine (match d2 with 
-      | (u,q1) => fun Hd2 => let (d3,Hd3) := fifo_3q_deq_full q1 _ 
+      | (u,q1) => fun Hd2 => let (d3,Hd3) := fifo_deq q1 _ 
                              in  _ 
     end).
     all: cycle 1.
     revert Hd3; refine (match d3 with
-      | (v,q2) => fun Hd3 => let (q3,Hq3) := fifo_3q_enq_full q2 (node v y u) 
+      | (v,q2) => fun Hd3 => let (q3,Hq3) := fifo_enq q2 (node v y u) 
                              in  exist _ q3 _
     end).
     all: cycle 1.
 
     * revert Hll; rewrite Hq; simpl.
-      generalize (fifo_3q_list p).
+      generalize (fifo_list p).
       intros [ | [] ? ]; simpl; try discriminate.
       split; auto.
       rewrite bft_f_fix_0; auto.
@@ -95,71 +98,69 @@ Section bfr_3q.
   
   Section bfr.
 
-    Let bfr_3q_full (t : bt X) (l : list Y) : m_bt t = length l -> { t' | t ~t t' /\ bft_std t' = l }.
+    Let bfr_gen_full (t : bt X) (l : list Y) : m_bt t = length l -> { t' | t ~t t' /\ bft_std t' = l }.
     Proof.
       intros H.
-      refine (match @bfr_3q_f (fifo_3q_enq fifo_3q_nil t) l _ with 
-        | exist _ q Hq => let (d1,Hd1) := fifo_3q_deq_full q _ in _ 
-      end).
+      refine (let (p,Hp) := @fifo_nil _     in
+              let (q,Hq) := fifo_enq p t    in 
+              let (r,Hr) := bfr_gen_f q l _ in
+              let (d1,Hd1) := fifo_deq r _ 
+              in _).
       all: cycle 2.
       revert Hd1; refine(match d1 with
         | (t',q') => fun Hd1 => exist _ t' _
       end).
       all: cycle 1.
 
-      + unfold fifo_3q_sum; rewrite fifo_3q_enq_spec, fifo_3q_nil_spec; simpl; omega.
-      + intros E; rewrite E in Hq; apply proj2 in Hq; simpl in Hq.
-        rewrite bft_f_fix_0 in Hq; subst.
+      + unfold fifo_sum.
+        rewrite Hq, Hp, <- H; simpl; omega.
+      + intros E; rewrite E in Hr; apply proj2 in Hr; simpl in Hr.
+        rewrite bft_f_fix_0 in Hr; subst.
         generalize (m_bt_ge_1 t); simpl in *; omega.
-      + destruct Hq as (Hq_1 & Hq_2); simpl in Hd1.
-        apply Forall2_rev in Hq_1.
-        rewrite fifo_3q_enq_spec, fifo_3q_nil_spec, rev_involutive, Hd1 in Hq_1; simpl in Hq_1.
-        apply Forall2_cons_inv in Hq_1.
-        destruct Hq_1 as (Hq_3 & Hq_1).
-        apply Forall2_nil_inv_right in Hq_1.
+      + destruct Hr as (Hr_1 & Hr_2); simpl in Hd1.
+        apply Forall2_rev in Hr_1.
+        rewrite Hq, Hp, rev_involutive, Hd1 in Hr_1; simpl in Hr_1.
+        apply Forall2_cons_inv in Hr_1.
+        destruct Hr_1 as (Hr_3 & Hr_1).
+        apply Forall2_nil_inv_right in Hr_1.
         split; auto.
-        rewrite Hd1, Hq_1 in Hq_2.
-        simpl in Hq_2.
+        rewrite Hd1, Hr_1 in Hr_2.
+        simpl in Hr_2.
         rewrite <- bft_std_eq_bft; auto.
     Qed.
 
-    Definition bfr_3q t l H := proj1_sig (bfr_3q_full t l H).
+    Definition bfr_gen t l H := proj1_sig (bfr_gen_full t l H).
 
-    Fact bfr_3q_spec_1 t l H : t ~t bfr_3q t l H.
-    Proof. apply (proj2_sig (bfr_3q_full t l H)). Qed.
+    Fact bfr_gen_spec_1 t l H : t ~t bfr_gen t l H.
+    Proof. apply (proj2_sig (bfr_gen_full t l H)). Qed.
 
-    Fact bfr_3q_spec_2 t l H : bft_std (bfr_3q t l H) = l.
-    Proof. apply (proj2_sig (bfr_3q_full t l H)). Qed.
+    Fact bfr_gen_spec_2 t l H : bft_std (bfr_gen t l H) = l.
+    Proof. apply (proj2_sig (bfr_gen_full t l H)). Qed.
 
   End bfr.
 
-End bfr_3q.
+End bfr_gen.
 
-(** BFN (Breadth-First Numbering) is a particular instance of 
-    BFR (Breadth-First Reconstruction)   *)
-
-Theorem bfr_bfn_3q X (t : bt X) : bfn_3q t = bfr_3q t (seq_an 0 (m_bt t)) (eq_sym (seq_an_length _ _)).
+Theorem bfr_bfn_gen X (t : bt X) : bfn_gen t = bfr_gen t (seq_an 0 (m_bt t)) (eq_sym (seq_an_length _ _)).
 Proof.
   apply bft_std_inj.
   * apply bt_eq_trans with (s := t).
-    + apply bt_eq_sym, bfn_3q_spec_1.
-    + apply bfr_3q_spec_1.
-  * rewrite bfr_3q_spec_2, bfn_3q_spec_3; trivial.
+    + apply bt_eq_sym, bfn_gen_spec_1.
+    + apply bfr_gen_spec_1.
+  * rewrite bfr_gen_spec_2, bfn_gen_spec_3; trivial.
 Qed.
-
-(* Notice that fifo_3q_deq is extracted to a function that loops forever
-   if the input is the empty queue, ie does not following the spec *)
 
 Extract Inductive bool => "bool" [ "true" "false" ].
 Extract Inductive prod => "(*)"  [ "(,)" ].
 Extract Inductive list => "list" [ "[]" "(::)" ].
 Extract Inductive nat => int [ "0" "succ" ] "(fun fO fS n -> if n=0 then fO () else fS (n-1))".
 
-Recursive Extraction bfr_3q.
+Recursive Extraction bfr_gen.
 
-Check bfr_3q.
-Check bfr_3q_spec_1.
-Check bfr_3q_spec_2.
-Check bfr_bfn_3q.
-             
+Check bfr_gen.
+Check bfr_gen_spec_1.
+Check bfr_gen_spec_2.
+
+(** BFN (Breadth-First Numbering) is a particular instance of 
+    BFR (Breadth-First Reconstruction)   *)
 
