bft_inj.v
@@ -1,0 +1,55 @@
+(**************************************************************)
+(*   Copyright Dominique Larchey-Wendling [*]                 *)
+(*                                                            *)
+(*                             [*] Affiliation LORIA -- CNRS  *)
+(**************************************************************)
+(*      This file is distributed under the terms of the       *)
+(*         CeCILL v2 FREE SOFTWARE LICENSE AGREEMENT          *)
+(**************************************************************)
+
+Require Import List Arith Omega Wellfounded Permutation.
+Require Import list_utils wf_utils bt bft.
+
+Set Implicit Arguments.
+
+Section bft_inj.
+
+  Variable X : Type.
+
+  Implicit Types (l : list (bt X)) (t : bt X).
+
+  Theorem bft_f_inj l m : l ~lt m -> bft_f l = bft_f m -> l = m.
+  Proof.
+    induction on l m as IH with measure (lsum (l++m)).
+    revert l m IH; intros [ | t1 l ] [ | t2 m ] IH H; try (inversion H; fail); auto.
+    Forall2 inv H as H12.
+    repeat rewrite bft_f_fix_3.
+    destruct t1 as [ x | a1 x b1 ]; destruct t2 as [ y | a2 y b2 ]; try (inversion H12; fail); simpl.
+    + intros E; inversion E; f_equal.
+      repeat rewrite <- app_nil_end in *.
+      apply IH; auto.
+      repeat rewrite lsum_app; simpl; omega.
+    + apply bt_eq_node_inv in H12; destruct H12 as [ Ha Hb ].
+      intros E; injection E; clear E; intros E ?; subst.
+      apply IH in E.
+      * apply f_equal with (f := @rev _) in E.
+        repeat rewrite rev_app_distr in E; simpl in E.
+        inversion E; subst; f_equal.
+        rewrite <- (rev_involutive l), <- (rev_involutive m).
+        f_equal; trivial.
+      * repeat rewrite lsum_app; simpl; omega.
+      * apply Forall2_app; auto.
+  Qed.
+
+  Corollary bft_inj t1 t2 : t1 ~t t2 -> bft t1 = bft t2 -> t1 = t2.
+  Proof.
+    unfold bft.
+    intros H1 H2. 
+    apply bft_f_inj in H2; auto.
+    inversion H2; auto.
+  Qed.
+
+  Corollary bft_std_inj t1 t2 : t1 ~t t2 -> bft_std t1 = bft_std t2 -> t1 = t2.
+  Proof. do 2 rewrite <- bft_std_eq_bft; apply bft_inj. Qed.
+
+End bft_inj.
