bt.v
@@ -33,6 +33,9 @@ Section bt.
       | node a _ b => 1 + m_bt a + m_bt b
     end.
 
+  Fact m_bt_ge_1 t : 1 <= m_bt t.
+  Proof. destruct t; simpl; omega. Qed.
+
   (* A branch is a list of left/right Boolean choices *)
 
   (* The branches that correspond to a node in a binary tree *)
@@ -197,13 +200,25 @@ Section bt_eq.
   Fact bt_eq_m t1 t2 : t1 ~t t2 -> m_bt t1 = m_bt t2.
   Proof. induction 1; simpl; f_equal; auto. Qed.
 
+  Fact bt_eq_node_inv a x b c y d : node a x b ~t node c y d -> a ~t c /\ b ~t d.
+  Proof. inversion 1; auto. Qed.
+
 End bt_eq.
 
 Arguments bt_eq {X Y}.
 
 Notation "x ~t y" := (bt_eq x y).
-Notation "l ~lt m" := (Forall2 bt_eq l m).
+Notation "l ~lt m" := (Forall2 bt_eq l m). (** extension to forests *)
 
 Hint Constructors bt_eq.
+
+Fact bt_eq_refl X (t : bt X) : t ~t t.
+Proof. induction t; constructor; auto. Qed.
+
+Fact bt_eq_sym X Y (s : bt X) (t : bt Y) : s ~t t -> t ~t s.
+Proof. induction 1; constructor; auto. Qed.
+
+Fact bt_eq_trans X Y Z (r : bt X) (s : bt Y) (t : bt Z) : r ~t s -> s ~t t -> r ~t t.
+Proof. intros H; revert H t; induction 1; inversion 1; auto. Qed.
 
 
