fifo_axm.v
@@ -22,3 +22,6 @@ Parameters (fifo      : Type -> Type)
            (fifo_enq  : forall X q x, { q' : fifo X | fifo_list q' = fifo_list q ++ x :: nil })
            (fifo_deq  : forall X q, @fifo_list X q <> nil -> { c : X * fifo X | let (x,q') := c in fifo_list q = x::fifo_list q' })
            (fifo_void : forall X q, { b : bool | b = true <-> @fifo_list X q = nil }).
+
+Arguments fifo_nil {X}.
+Arguments fifo_deq {X}.
